src/hls/ClockMemoryproof.v
@@ -53,18 +53,29 @@ Inductive match_reg_assocs : reg_associations -> reg_associations -> Prop :=
       match_assocmaps ran ran' ->
       match_reg_assocs (mkassociations rab ran) (mkassociations rab' ran').
 
+Inductive match_arr_sizes : assocmap_arr -> reg -> nat -> Prop :=
+| match_arr_sizes_intro : forall arr stk stk_arr len,
+  arr ! stk = Some stk_arr ->
+  arr_length stk_arr = len ->
+  match_arr_sizes arr stk len.
+
 Inductive match_stackframes : stackframe -> stackframe -> Prop :=
   match_stackframe_intro :
-    forall r m pc asr asa asr'
-      (MATCH_ASSOC: match_assocmaps asr asr'),
+    forall r m pc asr asa asr' asa'
+      (STK_ASSOC: match_assocmaps asr asr')
+      (STK_ARR_ASSOC: match_arrs asa asa')
+      (STK_ARR_SIZE1: match_empty_size m asa)
+      (STK_ARR_SIZE2: match_empty_size m asa'),
       match_stackframes (Stackframe r m pc asr asa)
-                        (Stackframe r (transf_module m) pc asr' asa).
+                        (Stackframe r (transf_module m) pc asr' asa').
 
 Inductive match_states : state -> state -> Prop :=
 | match_state :
     forall res res' m st asr asr' asa asa'
            (ASSOC: match_assocmaps asr asr')
-           (ASSOC': match_arrs asa asa')
+           (ARR_ASSOC: match_arrs asa asa')
+           (ARR_SIZE1: match_empty_size m asa)
+           (ARR_SIZE2: match_empty_size m asa')
            (STACK: Forall2 match_stackframes res res'),
       match_states (State res m st asr asa)
                    (State res' (transf_module m) st asr' asa')
@@ -130,7 +141,7 @@ Proof. inversion 1. auto. Qed.
 
 Lemma match_assocmaps_inv_map :
   forall a b, match_assocmaps a b -> forall x n, b # (x, n) = a # (x, n).
-Proof. 
+Proof.
   inversion 1; subst; intros.
   unfold find_assocmap, AssocMapExt.get_default.
   now rewrite H0.
@@ -169,224 +180,404 @@ Proof.
   - inv H. rewrite !AssocMap.gso by auto. eauto.
 Qed.
 
-Lemma expr_runp_same :
-  forall f rs1 ar1 c v,
-    expr_runp f rs1 ar1 c v ->
-    forall trs1,
-      match_assocmaps rs1 trs1 ->
-      expr_runp f trs1 ar1 c v.
+Lemma expr_interchangeable:
+  forall e r v a ar f v',
+    check_excluded r e = true ->
+    expr_runp f a ar e v ->
+    expr_runp f (AssocMap.set r v' a) ar e v.
 Proof.
-  induction 1; intros.
-  - econstructor.
-  - econstructor. erewrite match_assocmaps_inv_map; eauto.
-  - exploit IHexpr_runp; eauto; intros. econstructor; eauto.
-  - exploit IHexpr_runp1; eauto; exploit IHexpr_runp2; eauto; intros.
-    econstructor; eauto.
-  - exploit IHexpr_runp; eauto; intros. econstructor; eauto.
-  - exploit IHexpr_runp1; eauto; exploit IHexpr_runp2; eauto; intros.
-    econstructor; eauto.
-  - exploit IHexpr_runp1; eauto; exploit IHexpr_runp2; eauto; intros.
-    eapply erun_Vternary_false; eauto.
-  - exploit IHexpr_runp; eauto; intros. econstructor; eauto.
+  induction e; intros; cbn in *; simplify; try rewrite negb_true_iff in *;
+  repeat match goal with | H: _ =? _ = false |- _ => apply Pos.eqb_neq in H end; inv H0; try solve [econstructor; eauto].
+  - econstructor; now rewrite assocmap_gso by auto.
+  - econstructor; eauto; now rewrite assocmap_gso by auto.
+Qed.
+
+Lemma expr_interchangeable2:
+  forall e r v a ar f v',
+    check_excluded r e = true ->
+    expr_runp f (AssocMap.set r v' a) ar e v ->
+    expr_runp f a ar e v.
+Proof.
+  induction e; intros; cbn in *; simplify; try rewrite negb_true_iff in *;
+  repeat match goal with | H: _ =? _ = false |- _ => apply Pos.eqb_neq in H end; inv H0; try solve [econstructor; eauto].
+  - econstructor; now rewrite assocmap_gso by auto.
+  - econstructor; eauto; now rewrite assocmap_gso by auto.
+Qed.
+
+Lemma expr_interchangeable3:
+  forall e r t asr iv v arr v',
+    check_excluded r e = true ->
+    expr_runp t asr (arr_assocmap_set r (valueToNat iv) v arr) e v' ->
+    expr_runp t asr arr e v'.
+Proof.
+  induction e; intros; cbn in *; simplify; try rewrite negb_true_iff in *;
+  repeat match goal with | H: _ =? _ = false |- _ => apply Pos.eqb_neq in H end; inv H0; try solve [econstructor; eauto].
+  econstructor; eauto. unfold arr_assocmap_lookup in *. unfold arr_assocmap_set in *.
+  destruct (arr ! r0) eqn:?; auto. rewrite AssocMap.gso in H9 by auto. auto.
+Qed.
+
+  (* Lemma transf_maps_correct': *)
+  (*   forall t asr asa s asr' asa', *)
+  (*     stmnt_runp t (mkassociations asr empty_assocmap) asa s asr' asa' -> *)
+  (*     (forall r e1 e0 r0 e3, s <> (Vseq (Vseq Vskip (Vblock (Vvari r e1) e0)) (Vblock (Vvar r0) e3))) -> *)
+  (*     forall tasr, *)
+  (*       match_reg_assocs (mkassociations asr empty_assocmap) (mkassociations tasr empty_assocmap) -> *)
+  (*       exists tasr', stmnt_runp t (mkassociations tasr empty_assocmap) asa (transf_maps s) tasr' asa' *)
+  (*                     /\ match_assocmaps (Verilog.merge_regs (assoc_nonblocking asr') (assoc_blocking asr')) *)
+  (*                     (Verilog.merge_regs (assoc_nonblocking tasr') (assoc_blocking tasr')). *)
+  (* Proof. *)
+  (*   intros * ? HNEQ **. destruct s; try solve [exploit match_states_same; eauto; simplify; *)
+  (*     exploit match_assocmaps_merge; eauto]. *)
+  (*   cbn in *.  *)
+  (*   repeat (destruct_match; try solve [exploit match_states_same; eauto; simplify; *)
+  (*     exploit match_assocmaps_merge; eauto]). *)
+  (*   - simplify. *)
+  (*     inv H. inv H11. inv H10. inv H14; inv H10. inv H15; inv H10. *)
+  (*     inv H14. *)
+  (*     eexists; split. econstructor. econstructor. econstructor. *)
+  (*     2: { econstructor. econstructor. econstructor. unfold block_reg in *; cbn in *. eapply expr_interchangeable; eauto. *)
+  (*          eapply expr_runp_same; eauto. inv H0; auto. eauto. } *)
+  (*     unfold block_reg in *; cbn in *. eapply expr_interchangeable2; eauto. *)
+  (*     eapply expr_runp_same; eauto. eapply match_assocmaps_set; eauto. *)
+  (*     inv H0; auto. *)
+  (*     econstructor; intros. cbn. *)
+  (*     unfold merge_regs, AssocMapExt.merge. inv H0; subst; cbn. *)
+  (*     rewrite !PTree.gcombine by auto. *)
+  (*     rewrite negb_true_iff in *. *)
+  (*     apply Pos.eqb_neq in H4. apply Pos.eqb_neq in H2. apply Pos.eqb_neq in H5. *)
+  (*     destruct (peq r r2); subst. *)
+  (*     + rewrite !AssocMap.gss by auto. rewrite !AssocMap.gso by auto. auto. *)
+  (*     + rewrite !AssocMap.gso by auto. *)
+  (*       destruct (peq r r1); subst. *)
+  (*       ** rewrite !AssocMap.gss. rewrite !AssocMap.gso by auto. auto. *)
+  (*       ** rewrite !AssocMap.gso by auto. inv H8. rewrite H. auto. *)
+  (*   - subst. exfalso; eapply HNEQ; eauto. *)
+  (* Qed. *)
+
+Lemma expr_runp_same :
+  forall f rs ar e v,
+    expr_runp f rs ar e v ->
+    forall trs tar,
+      match_assocmaps rs trs ->
+      match_arrs ar tar ->
+      expr_runp f trs tar e v.
+Proof.
+  induction 1.
+  - intros. econstructor.
+  - intros. econstructor. inv H0. symmetry.
+    apply find_assoc_get.
+    apply H2.
+  - intros. econstructor. apply IHexpr_runp; eauto.
+    inv H2.
+    unfold arr_assocmap_lookup in *.
+    destruct (stack ! r) eqn:?; [|discriminate].
+    inv H0.
+    eapply H3 in Heqo. inv Heqo. inv H0.
+    unfold arr in *. rewrite H2. inv H5.
+    rewrite H0. auto.
+  - intros. econstructor; eauto.
+  - intros. econstructor; eauto.
+  - intros. econstructor; eauto.
+  - intros. eapply erun_Vternary_false. apply IHexpr_runp1; eauto.
+    apply IHexpr_runp2; eauto. auto.
+  - intros. econstructor. apply IHexpr_runp; eauto. eauto. eauto.
     erewrite match_assocmaps_inv_map; eauto. rewrite H0. now rewrite H1.
 Qed.
 
-Lemma match_states_same :
+Lemma stmnt_runp_same :
   forall f rs1 ar1 c rs2 ar2,
     stmnt_runp f rs1 ar1 c rs2 ar2 ->
-    forall trs1,
-      match_reg_assocs rs1 trs1 ->
-      exists trs2,
-        stmnt_runp f trs1 ar1 c trs2 ar2
-        /\ match_reg_assocs rs2 trs2.
+      forall trs1 tar1,
+        match_reg_assocs rs1 trs1 ->
+        match_arr_assocs ar1 tar1 ->
+        exists trs2 tar2,
+          stmnt_runp f trs1 tar1 c trs2 tar2
+          /\ match_reg_assocs rs2 trs2
+          /\ match_arr_assocs ar2 tar2.
 Proof.
   induction 1.
-  - econstructor; split; eauto; constructor.
-  - intros. exploit IHstmnt_runp1; eauto; simplify. 
+  - do 2 eexists; split; [|split]; eauto; constructor.
+  - intros. exploit IHstmnt_runp1; eauto; simplify.
     exploit IHstmnt_runp2; eauto; simplify.
-    econstructor; split.
-    + econstructor; eauto.
-    + auto.
+    do 2 econstructor; split; [|split]; eauto.
+    econstructor; eauto.
   - intros. exploit IHstmnt_runp; eauto; simplify.
-    inversion H2; subst; exploit expr_runp_same; eauto; intros.
-    eexists; split; eauto; econstructor; eauto.
+    inversion H2; inversion H3; subst; exploit expr_runp_same; eauto; intros.
+    do 2 eexists; split; eauto; econstructor; eauto.
   - intros. exploit IHstmnt_runp; eauto; simplify.
-    inversion H2; subst; exploit expr_runp_same; eauto; intros.
-    eexists; split; eauto; eapply stmnt_runp_Vcond_false; eauto.
+    inversion H2; inversion H3; subst; exploit expr_runp_same; eauto; intros.
+    do 2 eexists; split; eauto; eapply stmnt_runp_Vcond_false; eauto.
   - intros. exploit IHstmnt_runp; eauto; simplify.
-    inversion H3. subst. exploit expr_runp_same; [eapply H| |]; eauto; intros.
-    exploit expr_runp_same; [eapply H0| |]; eauto; intros.
-    eexists; split; eauto. econstructor; eauto.
+    inversion H3; inversion H4. subst. exploit expr_runp_same; [eapply H| | |]; eauto; intros.
+    exploit expr_runp_same; [eapply H0| | |]; eauto; intros.
+    do 2 eexists; split; eauto. econstructor; eauto.
   - intros. exploit IHstmnt_runp; eauto; simplify.
-    inversion H3. subst. exploit expr_runp_same; [eapply H| |]; eauto; intros.
-    exploit expr_runp_same; [eapply H0| |]; eauto; intros.
-    eexists; split; eauto. eapply stmnt_runp_Vcase_match; eauto.
+    inversion H3; inversion H4; subst. exploit expr_runp_same; [eapply H| | |]; eauto; intros.
+    exploit expr_runp_same; [eapply H0| | |]; eauto; intros.
+    do 2 eexists; split; eauto. eapply stmnt_runp_Vcase_match; eauto.
   - intros. exploit IHstmnt_runp; eauto; simplify.
-    inversion H1. subst. exploit expr_runp_same; [eapply H| |]; eauto; intros.
-    eexists; split; eauto. eapply stmnt_runp_Vcase_default; eauto.
+    inversion H1; inversion H2. subst. exploit expr_runp_same; [eapply H| | |]; eauto; intros.
+    do 2 eexists; split; eauto. eapply stmnt_runp_Vcase_default; eauto.
   - inv H; intros.
-    inversion H. subst. exploit expr_runp_same; eauto; intros.
-    econstructor; split; intros. econstructor; eauto. econstructor.
-    econstructor; cbn; eauto.
-    econstructor; intros.
-    destruct (peq r r0); subst.
-    + now rewrite !AssocMap.gss.
-    + rewrite !AssocMap.gso by auto. inv H1; eauto.
-  - inv H; intros.
-    inversion H. subst. exploit expr_runp_same; eauto; intros.
-    econstructor; split; intros. econstructor; eauto. econstructor.
+    inversion H; inversion H1; subst. exploit expr_runp_same; eauto; intros.
+    do 2 econstructor; split; [|split]; intros. econstructor; eauto. econstructor.
     econstructor; cbn; eauto.
     econstructor; intros.
     destruct (peq r r0); subst.
     + now rewrite !AssocMap.gss.
     + rewrite !AssocMap.gso by auto. inv H2; eauto.
-  - inv H; intros. inversion H; subst.
-    exploit expr_runp_same; [eapply H0| |]; eauto; intros.
-    exploit expr_runp_same; [eapply H6| |]; eauto; intros.
-    eexists; split; eauto. econstructor; eauto. econstructor; eauto.
-  - inv H; intros. inversion H; subst.
-    exploit expr_runp_same; [eapply H0| |]; eauto; intros.
-    exploit expr_runp_same; [eapply H6| |]; eauto; intros.
-    eexists; split; eauto. econstructor; eauto. econstructor; eauto.
+    + eauto.
+  - inv H; intros.
+    inversion H; inversion H1; subst. exploit expr_runp_same; eauto; intros.
+    do 2 econstructor; split; [|split]; intros. econstructor; eauto. econstructor.
+    econstructor; cbn; eauto.
+    econstructor; intros.
+    destruct (peq r r0); subst.
+    + now rewrite !AssocMap.gss.
+    + rewrite !AssocMap.gso by auto. inv H3; eauto.
+    + eauto.
+  - inv H; intros. inversion H; inversion H1; subst.
+    exploit expr_runp_same; [eapply H0| | |]; eauto; intros.
+    exploit expr_runp_same; [eapply H6| | |]; eauto; intros.
+    do 2 eexists; split; [|split]; eauto.
+    econstructor; eauto. econstructor; eauto.
+    eapply match_arr_assocs_block; eauto.
+  - inv H; intros. inversion H; inversion H1; subst.
+    exploit expr_runp_same; [eapply H0| | |]; eauto; intros.
+    exploit expr_runp_same; [eapply H6| | |]; eauto; intros.
+    do 2 eexists; split; [|split]; eauto.
+    econstructor; eauto. econstructor; eauto.
+    eapply match_arr_assocs_nonblock; eauto.
 Qed.
 
 Lemma exec_ram_same :
   forall rs1 ar1 c rs2 ar2,
     exec_ram rs1 ar1 c rs2 ar2 ->
-    forall trs1,
+    forall trs1 tar1,
       match_reg_assocs rs1 trs1 ->
-      exists trs2,
-        exec_ram trs1 ar1 c trs2 ar2
-        /\ match_reg_assocs rs2 trs2.
+      match_arr_assocs ar1 tar1 ->
+      exists trs2 tar2,
+        exec_ram trs1 tar1 c trs2 tar2
+        /\ match_reg_assocs rs2 trs2
+        /\ match_arr_assocs ar2 tar2.
 Proof.
   induction 1; intros.
-  - eexists; split; eauto.
+  - do 2 eexists; split; [|split]; eauto.
     apply exec_ram_Some_idle. inv H0. cbn in *; setoid_rewrite match_assocmaps_inv_map; eauto.
-  - inv H6; eexists; split; cbn in *.
+  - inv H6; do 2 eexists; split; [|split]; cbn in *.
     + eapply exec_ram_Some_write. eapply H. eauto. all: cbn in *.
       now erewrite match_assocmaps_inv_map by eauto.
-      all: now erewrite match_assocmaps_inv by eauto.
+      all: try (erewrite match_assocmaps_inv by eauto; eauto).
     + unfold nonblock_reg; cbn. constructor; auto.
       now apply match_assocmaps_set.
-  - inv H5; eexists; split; cbn in *.
+    + eapply match_arr_assocs_nonblock; eauto.
+  - inv H5; do 2 eexists; split; [|split]; cbn in *.
     + eapply exec_ram_Some_read; eauto; cbn in *.
       now erewrite match_assocmaps_inv_map by eauto.
-      all: now erewrite match_assocmaps_inv by eauto.
+      all: (try (erewrite match_assocmaps_inv by eauto; eauto)).
+      eapply match_arrs_read; eauto. inv H6; eauto.
     + unfold nonblock_reg; cbn. constructor; auto.
       now repeat apply match_assocmaps_set.
-  - eexists; split; cbn in *; eauto. econstructor.
+    + eauto.
+  - do 2 eexists; split; [|split]; cbn in *; eauto. econstructor.
 Qed.
 
-  Lemma expr_interchangeable:
-    forall e r v a ar f v',
-      check_excluded r e = true ->
-      expr_runp f a ar e v ->
-      expr_runp f (AssocMap.set r v' a) ar e v.
-  Proof. 
-    induction e; intros; cbn in *; simplify; try rewrite negb_true_iff in *;
-    repeat match goal with | H: _ =? _ = false |- _ => apply Pos.eqb_neq in H end; inv H0; try solve [econstructor; eauto].
-    - econstructor; now rewrite assocmap_gso by auto.
-    - econstructor; eauto; now rewrite assocmap_gso by auto.
-  Qed.
+Lemma match_reg_assocs_empty :
+  forall ars ars',
+    match_assocmaps ars ars' ->
+    match_reg_assocs (mkassociations ars empty_assocmap) (mkassociations ars' empty_assocmap).
+Proof.
+  intros; constructor; auto.
+  apply match_assocmaps_refl.
+Qed.
 
-  Lemma expr_interchangeable2:
-    forall e r v a ar f v',
-      check_excluded r e = true ->
-      expr_runp f (AssocMap.set r v' a) ar e v ->
-      expr_runp f a ar e v.
-  Proof. 
-    induction e; intros; cbn in *; simplify; try rewrite negb_true_iff in *;
-    repeat match goal with | H: _ =? _ = false |- _ => apply Pos.eqb_neq in H end; inv H0; try solve [econstructor; eauto].
-    - econstructor; now rewrite assocmap_gso by auto.
-    - econstructor; eauto; now rewrite assocmap_gso by auto.
-  Qed.
+Lemma match_arr_assocs_empty :
+  forall ars ars',
+    match_arrs ars ars' ->
+    forall st l, match_arr_assocs (mkassociations ars (empty_stack st l)) 
+                   (mkassociations ars' (empty_stack st l)).
+Proof.
+  intros; constructor; auto. apply match_arrs_equiv.
+Qed.
 
-  Lemma expr_interchangeable3:
-    forall e r t asr iv v arr v',
-      check_excluded r e = true ->
-      expr_runp t asr (arr_assocmap_set r (valueToNat iv) v arr) e v' ->
-      expr_runp t asr arr e v'.
+Lemma match_empty_size_empty_stack:
+  forall m, match_empty_size m (empty_stack (mod_stk m) (mod_stk_len m)).
+Proof.
+  unfold match_empty_size; intros.
+  apply match_arrs_size_equiv.
+Qed.
+
+Lemma match_arrs_trans :
+  forall asa1 asa2 asa3, 
+    match_arrs asa1 asa2 -> match_arrs asa2 asa3 -> match_arrs asa1 asa3.
+Proof.
+  inversion 1. inversion 1; subst.
+  econstructor; eauto.
+  intros. eapply H0 in H2. simplify. eapply H5 in H2; simplify.
+  econstructor; split; eauto. split; congruence.
+Qed.
+
+
+  Lemma arr_assocmap_set_gss :
+    forall r i v asa ar,
+      asa ! r = Some ar ->
+      (arr_assocmap_set r i v asa) ! r = Some (array_set i (Some v) ar).
   Proof.
-    induction e; intros; cbn in *; simplify; try rewrite negb_true_iff in *;
-    repeat match goal with | H: _ =? _ = false |- _ => apply Pos.eqb_neq in H end; inv H0; try solve [econstructor; eauto].
-    econstructor; eauto. unfold arr_assocmap_lookup in *. unfold arr_assocmap_set in *.
-    destruct (arr ! r0) eqn:?; auto. rewrite AssocMap.gso in H9 by auto. auto.
+    unfold arr_assocmap_set.
+    intros. rewrite H. rewrite PTree.gss. auto.
   Qed.
 
-  Lemma transf_maps_correct:
-    forall t asr asa s asr' asa',
-      stmnt_runp t (mkassociations asr empty_assocmap) asa s asr' asa' ->
-      (forall r e1 e0 r0 e3, s <> (Vseq (Vseq Vskip (Vblock (Vvari r e1) e0)) (Vblock (Vvar r0) e3))) ->
-      forall tasr,
-        match_reg_assocs (mkassociations asr empty_assocmap) (mkassociations tasr empty_assocmap) ->
-        exists tasr', stmnt_runp t (mkassociations tasr empty_assocmap) asa (transf_maps s) tasr' asa'
-                      /\ match_assocmaps (Verilog.merge_regs (assoc_nonblocking asr') (assoc_blocking asr'))
-                      (Verilog.merge_regs (assoc_nonblocking tasr') (assoc_blocking tasr')).
+  Lemma arr_assocmap_set_gso :
+    forall r x i v asa ar,
+      asa ! x = Some ar ->
+      r <> x ->
+      (arr_assocmap_set r i v asa) ! x = asa ! x.
   Proof.
-    intros * ? HNEQ **. destruct s; try solve [exploit match_states_same; eauto; simplify;
-      exploit match_assocmaps_merge; eauto].
-    cbn in *. 
-    repeat (destruct_match; try solve [exploit match_states_same; eauto; simplify;
-      exploit match_assocmaps_merge; eauto]).
-    - simplify.
-      inv H. inv H11. inv H10. inv H14; inv H10. inv H15; inv H10.
-      inv H14.
-      eexists; split. econstructor. econstructor. econstructor.
-      2: { econstructor. econstructor. econstructor. unfold block_reg in *; cbn in *. eapply expr_interchangeable; eauto.
-           eapply expr_runp_same; eauto. inv H0; auto. eauto. }
-      unfold block_reg in *; cbn in *. eapply expr_interchangeable2; eauto.
-      eapply expr_runp_same; eauto. eapply match_assocmaps_set; eauto.
-      inv H0; auto.
-      econstructor; intros. cbn.
-      unfold merge_regs, AssocMapExt.merge. inv H0; subst; cbn.
-      rewrite !PTree.gcombine by auto.
-      rewrite negb_true_iff in *.
-      apply Pos.eqb_neq in H4. apply Pos.eqb_neq in H2. apply Pos.eqb_neq in H5.
-      destruct (peq r r2); subst.
-      + rewrite !AssocMap.gss by auto. rewrite !AssocMap.gso by auto. auto.
-      + rewrite !AssocMap.gso by auto.
+    unfold arr_assocmap_set. intros. 
+    destruct (asa!r) eqn:?; auto; now rewrite PTree.gso by auto.
+  Qed.
+
+  Lemma arr_assocmap_set_gs2 :
+    forall r x i v asa,
+      asa ! x = None ->
+      (arr_assocmap_set r i v asa) ! x = None.
+  Proof.
+    unfold arr_assocmap_set. intros. 
+    destruct (peq r x); subst; [now rewrite H|].
+    destruct (asa!r) eqn:?; auto.
+    now rewrite PTree.gso by auto.
+  Qed.
+
+  Lemma arr_assocmap_set_gs2' :
+    forall r x i v asa,
+      (arr_assocmap_set r i v asa) ! x = None ->
+      asa ! x = None.
+  Proof.
+    unfold arr_assocmap_set. intros. destruct_match; auto.
+    destruct (peq r x); subst.
+    - rewrite PTree.gss in H. inv H.
+    - now rewrite PTree.gso in H by auto.
+  Qed.
+
+Lemma transf_maps_correct:
+  forall t asr asa s asr' asa' m,
+    stmnt_runp t (mkassociations asr empty_assocmap) (mkassociations asa (empty_stack (mod_stk m) (mod_stk_len m))) s asr' asa' ->
+    forall tasr tasa,
+      match_assocmaps asr tasr ->
+      match_arrs asa tasa ->
+      match_empty_size m asa ->
+      match_empty_size m tasa ->
+      exists tasr' tasa',
+        stmnt_runp t (mkassociations tasr empty_assocmap) (mkassociations tasa (empty_stack (mod_stk m) (mod_stk_len m)))
+          (transf_maps (mod_stk m) s) tasr' tasa'
+        /\ match_assocmaps (Verilog.merge_regs (assoc_nonblocking asr') (assoc_blocking asr'))
+                           (Verilog.merge_regs (assoc_nonblocking tasr') (assoc_blocking tasr'))
+        /\ match_arrs (Verilog.merge_arrs (assoc_nonblocking asa') (assoc_blocking asa'))
+                      (Verilog.merge_arrs (assoc_nonblocking tasa') (assoc_blocking tasa')).
+Proof.
+  intros * HSTMNT * HMATCH_ASSOC HMATCH_ARR HMATCH_SIZE1 HMATCH_SIZE2. 
+  pose proof (match_reg_assocs_empty _ _ ltac:(eauto)) as HREG_ASSOCS;
+    pose proof (match_arr_assocs_empty _ _ ltac:(eauto)) as HARR_ASSOCS;
+    exploit stmnt_runp_same; eauto; intros (trs2 & tar2 & HSTMNT' & HMATCH_REG' & HMATCH_ARR');
+    pose proof (match_assocmaps_merge _ _ ltac:(eauto)) as HMATCH_MERGE_REG;
+    pose proof (match_empty_size_empty_stack m);
+    exploit match_arrs_size_stmnt_preserved; try exact HSTMNT'; eauto; cbn; 
+    intros (HMATCH_SZ_BLOCK' & HMATCH_SZ_NONBLOCK');
+    exploit match_arrs_size_stmnt_preserved; try exact HSTMNT; eauto; cbn; 
+    intros (HMATCH_SZ_BLOCK & HMATCH_SZ_NONBLOCK);
+    pose proof (match_empty_size_match _ _ _ HMATCH_SZ_BLOCK HMATCH_SZ_NONBLOCK) as MATCH_SIZE;
+    inversion HMATCH_ARR' as [basa' btar2 nasa' ntar2 HMATCH_ARR'1 HMATCH_ARR'2]; subst; cbn in *;
+    pose proof (match_arrs_merge _ _ _ _ MATCH_SIZE HMATCH_ARR'2 HMATCH_ARR'1) as MATCH_MERGE.
+  unfold transf_maps. repeat destruct_match; eauto; 
+  repeat (kill_bools; match goal with | H: _ /\ _ |- _ => inv H end);
+  try rewrite negb_true_iff in *;
+  repeat match goal with | H: _ =? _ = false |- _ => apply Pos.eqb_neq in H
+                         | H: _ =? _ = true |- _ => apply Pos.eqb_eq in H end; subst.
+  - rename H3 into NE1, H4 into NE2, H5 into NE3, H0 into CHECK1, H6 into CHECK2.
+    inv HSTMNT'. inv H5. inv H6. inv H8; [|inv H7]. inv H5. inv H10; inv H7.
+    inv H11. cbn in *.
+    do 2 eexists; split; [|split].
+    + econstructor. econstructor. econstructor. cbn. eapply expr_interchangeable2; eauto.
+      econstructor. econstructor. econstructor; cbn. eapply expr_interchangeable; eauto.
+      eassumption.
+    + cbn. eapply match_assocmaps_trans; eauto. econstructor; intros.
+      unfold merge_regs, AssocMapExt.merge, empty_assocmap. rewrite !PTree.gcombine by auto.
+      destruct (peq r r0); subst.
+      * rewrite !PTree.gss. rewrite PTree.gso by auto. now rewrite !PTree.gempty.
+      * repeat (rewrite !PTree.gso by auto; symmetry). setoid_rewrite PTree.gso at 2; auto.
         destruct (peq r r1); subst.
-        ** rewrite !AssocMap.gss. rewrite !AssocMap.gso by auto. auto.
-        ** rewrite !AssocMap.gso by auto. inv H8. rewrite H. auto.
-    - subst. exfalso; eapply HNEQ; eauto.
-  Qed.
-
-  Lemma transf_maps_correct2:
-    forall t asr asa s asr' asa',
-      stmnt_runp t (mkassociations asr empty_assocmap) asa s asr' asa' ->
-      (forall r e1 e0 r0 e3, s <> (Vseq (Vseq Vskip (Vblock (Vvari r e1) e0)) (Vblock (Vvar r0) e3))) ->
-      forall tasr,
-        match_reg_assocs (mkassociations asr empty_assocmap) (mkassociations tasr empty_assocmap) ->
-        exists tasr', stmnt_runp t (mkassociations tasr empty_assocmap) asa (transf_maps s) tasr' asa'
-                      /\ match_assocmaps (Verilog.merge_regs (assoc_nonblocking asr') (assoc_blocking asr'))
-                      (Verilog.merge_regs (assoc_nonblocking tasr') (assoc_blocking tasr')).
-  Proof.
-
-  Lemma transf_maps_correct2:
-    forall t asr asa r e1 e0 r0 e3 asr' asa' st l,
-      stmnt_runp t (mkassociations asr empty_assocmap) (mkassociations asa (empty_stack st l)) 
-        (Vseq (Vseq Vskip (Vblock (Vvari r e1) e0)) (Vblock (Vvar r0) e3)) asr' asa' ->
-      forall tasr,
-        match_reg_assocs (mkassociations asr empty_assocmap) (mkassociations tasr empty_assocmap) ->
-        exists tasr' tasa', stmnt_runp t (mkassociations tasr empty_assocmap) (mkassociations asa (empty_stack st l)) 
-                        (transf_maps (Vseq (Vseq Vskip (Vblock (Vvari r e1) e0)) (Vblock (Vvar r0) e3))) tasr' tasa'
-                      /\ match_assocmaps (Verilog.merge_regs (assoc_nonblocking asr') (assoc_blocking asr'))
-                      (Verilog.merge_regs (assoc_nonblocking tasr') (assoc_blocking tasr'))
-                      /\ Verilog.merge_arrs (assoc_nonblocking tasa') (assoc_blocking tasa') 
-                         = Verilog.merge_arrs (assoc_nonblocking asa') (assoc_blocking asa').
-  Proof.
-    intros; cbn in *. inv H0. clear H6.
-    inv H. inv H6. inv H5. inv H9; inv H5. inv H10; inv H5. cbn in *. destruct_match; cbn in *;
-    repeat (kill_bools; match goal with | H: _ /\ _ |- _ => inv H end).
-    - rewrite negb_true_iff in *. apply Pos.eqb_neq in H0. do 2 eexists; split; [|split].
-      + econstructor. econstructor. econstructor. cbn. eapply expr_interchangeable3; eauto.
-        eapply expr_runp_same; eauto.
-        eapply stmnt_runp_Vnonblock_arr. econstructor. 
-        cbn. eapply expr_interchangeable; eauto. eapply expr_runp_same; eauto.
-        cbn. eapply expr_interchangeable; eauto. eapply expr_runp_same; eauto.
-      + cbn. eapply match_assocmaps_merge2; eauto. apply match_assocmaps_refl.
-        now apply match_assocmaps_set.
-      + cbn. unfold merge_arrs.
+        -- rewrite PTree.gss. rewrite PTree.gempty. rewrite PTree.gss. auto.
+        -- rewrite !PTree.gso by auto. auto.
+    + auto.
+  - rename H3 into NE1, H4 into CHECK3, H2 into CHECK1, H5 into CHECK2.
+    inv HSTMNT'. inv H5. inv H6. inv H8; [|inv H7]. inv H5. inv H10; inv H7.
+    cbn in *.
+    do 2 eexists; split; [|split].
+    + econstructor. econstructor. econstructor. cbn. eapply expr_interchangeable3; eauto.
+      eapply stmnt_runp_Vnonblock_arr. econstructor. cbn. eapply expr_interchangeable; eauto.
+      eapply expr_interchangeable; eauto.
+    + cbn. eapply match_assocmaps_trans; eauto. econstructor; intros. auto.
+    + cbn. eapply match_arrs_trans; eauto.
+      econstructor; intros.
+      * eapply merge_arr_empty' in H0; [|eapply match_empty_assocmap_set; eauto].
+        destruct (peq s (mod_stk m)); subst.
+        -- exploit arrs_present; eauto; simplify. erewrite arr_assocmap_set_gss in H0; eauto.
+           inv H0. clear MATCH_MERGE.
+           eexists; split; [|split].
+           ** unfold merge_arrs. rewrite AssocMap.gcombine by auto.
+              unfold merge_arr. rewrite H2.
+              erewrite arr_assocmap_set_gss; eauto.
+              unfold empty_stack. rewrite PTree.gss. eauto.
+           ** intros.
+              inv HMATCH_SIZE2. eapply H1 in H2. simplify.
+              unfold empty_stack in H2. rewrite AssocMap.gss in H2. inv H2.
+              case_eq ((addr <? arr_length x)%nat); intros.
+              ++ pose proof (Nat.ltb_spec0 addr (arr_length x)). rewrite H2 in H5. inv H5.
+                 destruct (Nat.eq_dec addr (valueToNat iv)); subst.
+                 --- rewrite array_get_error_set_bound by auto.
+                     erewrite combine_lookup_second; eauto.
+                     now rewrite array_get_error_set_bound by lia.
+                 --- rewrite array_gso by auto. 
+                     erewrite combine_array_set; eauto.
+                     rewrite array_gso by auto. 
+                     rewrite arr_repeat_length in H6.
+                     now rewrite combine_none2 by auto.
+              ++ pose proof (Nat.ltb_spec0 addr (arr_length x)). rewrite H2 in H5. inv H5.
+                 assert ((addr >= arr_length x)%nat) by lia.
+                 pose proof (@arr_repeat_length (option value) (mod_stk_len m) None).
+                 pose proof (array_set_len x (valueToNat iv) (Some rhsval0)).
+                 assert (arr_length (array_set (valueToNat iv) (Some rhsval0) x) = arr_length (arr_repeat None (mod_stk_len m))) by eauto.
+                 exploit (@combine_length (option value)); eauto; intros.
+                 instantiate (1 := merge_cell) in H13.
+                 setoid_rewrite array_get_error_bound_gt; auto. 
+                 rewrite combine_length; eauto. 
+                 erewrite <- array_set_len; eauto.
+                 rewrite arr_repeat_length; eauto. lia.
+           ** inv HMATCH_SIZE2. eapply H1 in H2.
+              unfold empty_stack in H2. rewrite AssocMap.gss in H2. inv H2.
+              inv H5. inv H2.
+              erewrite <- array_set_len; eauto.
+              rewrite combine_length; eauto.
+        -- unfold merge_arrs. rewrite AssocMap.gcombine.
+           destruct (tasa ! s) eqn:?.
+           ** inv HMATCH_SIZE2. eapply H2 in Heqo. simplify. unfold empty_stack in H6.
+              rewrite PTree.gso in H6 by auto. now rewrite PTree.gempty in H6.
+           ** now rewrite arr_assocmap_set_gs2 in H0 by auto.
+           ** auto.
+      * unfold merge_arrs in *. rewrite AssocMap.gcombine in * by auto. unfold empty_stack in *.
+        destruct (peq s (mod_stk m)); subst.
+        -- rewrite AssocMap.gss in H0.
+           inv HMATCH_SIZE2; eauto. unfold empty_stack in *. 
+           assert ((AssocMap.set (mod_stk m) (arr_repeat None (mod_stk_len m)) (AssocMap.empty arr)) ! (mod_stk m) = Some (arr_repeat None (mod_stk_len m))) by (now rewrite AssocMap.gss by auto).
+           eapply H1 in H5. clear MATCH_MERGE; simplify.
+           now (erewrite arr_assocmap_set_gss in H0; eauto).
+        -- destruct (tasa ! s) eqn:?.
+           ** inv HMATCH_SIZE2; eauto. eapply H2 in Heqo.
+              clear MATCH_MERGE. simplify. unfold empty_stack in *.
+              rewrite AssocMap.gso in H6 by auto. now rewrite AssocMap.gempty in H6.
+           ** rewrite arr_assocmap_set_gs2; auto. rewrite AssocMap.gso by auto.
+              now rewrite AssocMap.gempty.
+Qed.
 
 Section CORRECTNESS.
 
@@ -434,27 +625,48 @@ Section CORRECTNESS.
       forall R1,
         match_states S1 R1 ->
         exists R2, step tge R1 t R2 /\ match_states S2 R2.
-  Proof. 
+  Proof.
     induction 1.
-    - inversion 1; subst. exploit transf_maps_correct; eauto. econstructor. eauto.
-      apply match_assocmaps_refl. intros ((btasr' & ntasr') & HSTMNT & HMATCH).
-      exploit exec_ram_same; eauto. econstructor; eauto. apply match_assocmaps_refl.
-      intros ((btrs2 & ntrs2) & HEXEC & HMATCH2).
-      econstructor. split. econstructor; cbn.
-      1-3: now erewrite match_assocmaps_inv by eauto.
-      rewrite PTree.gmap1. rewrite H2. cbn. auto. eassumption.
-      eassumption. eauto. eauto. eapply match_assocmaps_merge in HMATCH2.
-      erewrite match_assocmaps_inv; eauto. eauto.
-      econstructor; auto. eapply match_assocmaps_merge in HMATCH2. eauto.
+    - inversion 1; subst.
+      exploit transf_maps_correct; eauto. simplify.
+      exploit exec_ram_same; eauto. econstructor; eauto. eapply match_assocmaps_refl.
+      econstructor; eauto. eapply match_arrs_equiv.
+      simplify.
+      destruct x, x0, x1, x2. cbn in *.
+      econstructor; split.
+      + econstructor; cbn.
+        1-3: now erewrite match_assocmaps_inv by eauto.
+        rewrite PTree.gmap1. rewrite H2. cbn. eauto. eassumption.
+        eassumption. eauto. eauto. inv H10.
+        erewrite match_assocmaps_inv; eauto. eapply match_assocmaps_merge2; eauto.
+        eauto.
+     + exploit match_arrs_size_stmnt_preserved; try eapply H3; eauto; cbn.
+       eapply match_empty_size_empty_stack. simplify.
+       exploit match_arrs_size_ram_preserved2; try eapply H4; eauto.
+       eapply match_empty_size_empty_stack. 
+       eapply match_empty_size_merge; eauto. simplify.
+       exploit match_arrs_size_stmnt_preserved; eauto; cbn.
+       eapply match_empty_size_empty_stack. simplify.
+       exploit match_arrs_size_ram_preserved2; eauto.
+       eapply match_empty_size_empty_stack. 
+       eapply match_empty_size_merge; eauto. simplify.
+       econstructor. inv H10; eapply match_assocmaps_merge2; eauto.
+       inv H14. eapply match_arrs_merge; eauto. eapply match_empty_size_match; eauto.
+       eapply match_empty_size_merge; eauto.
+       eapply match_empty_size_merge; eauto.
+       eauto.
     - inversion 1; subst. econstructor; split.
       apply step_finish; cbn. now erewrite match_assocmaps_inv by eauto.
       erewrite match_assocmaps_inv by eauto. eassumption.
       econstructor; auto.
     - inversion 1; subst; intros. econstructor; split.
       apply step_call. econstructor; auto. inv H.
-      repeat apply match_assocmaps_set. cbn. 
+      repeat apply match_assocmaps_set. cbn.
       apply match_assocmaps_refl.
-    - inversion 1; subst. inv STACKS. inv H0. destruct y.  
+      cbn. apply match_arrs_equiv.
+      apply match_empty_size_empty_stack.
+      cbn; apply match_empty_size_empty_stack.
+    - inversion 1; subst. inv STACKS. inv H0. destruct y.
       eexists; split. eapply step_return. eauto. inv H2.
       constructor; auto. repeat apply match_assocmaps_set. auto.
   Qed.
