src/hls/ClockRegistersproof.v
@@ -1,0 +1,107 @@
+Lemma expr_runp_same :
+  forall f rs1 ar1 c v,
+    expr_runp f rs1 ar1 c v ->
+    forall trs1,
+      match_assocmaps rs1 trs1 ->
+      expr_runp f trs1 ar1 c v.
+Proof.
+  induction 1; intros.
+  - econstructor.
+  - econstructor. erewrite match_assocmaps_inv_map; eauto.
+  - exploit IHexpr_runp; eauto; intros. econstructor; eauto.
+  - exploit IHexpr_runp1; eauto; exploit IHexpr_runp2; eauto; intros.
+    econstructor; eauto.
+  - exploit IHexpr_runp; eauto; intros. econstructor; eauto.
+  - exploit IHexpr_runp1; eauto; exploit IHexpr_runp2; eauto; intros.
+    econstructor; eauto.
+  - exploit IHexpr_runp1; eauto; exploit IHexpr_runp2; eauto; intros.
+    eapply erun_Vternary_false; eauto.
+  - exploit IHexpr_runp; eauto; intros. econstructor; eauto.
+    erewrite match_assocmaps_inv_map; eauto. rewrite H0. now rewrite H1.
+Qed.
+
+Lemma match_states_same :
+  forall f rs1 ar1 c rs2 ar2,
+    stmnt_runp f rs1 ar1 c rs2 ar2 ->
+    forall trs1,
+      match_reg_assocs rs1 trs1 ->
+      exists trs2,
+        stmnt_runp f trs1 ar1 c trs2 ar2
+        /\ match_reg_assocs rs2 trs2.
+Proof.
+  induction 1.
+  - econstructor; split; eauto; constructor.
+  - intros. exploit IHstmnt_runp1; eauto; simplify. 
+    exploit IHstmnt_runp2; eauto; simplify.
+    econstructor; split.
+    + econstructor; eauto.
+    + auto.
+  - intros. exploit IHstmnt_runp; eauto; simplify.
+    inversion H2; subst; exploit expr_runp_same; eauto; intros.
+    eexists; split; eauto; econstructor; eauto.
+  - intros. exploit IHstmnt_runp; eauto; simplify.
+    inversion H2; subst; exploit expr_runp_same; eauto; intros.
+    eexists; split; eauto; eapply stmnt_runp_Vcond_false; eauto.
+  - intros. exploit IHstmnt_runp; eauto; simplify.
+    inversion H3. subst. exploit expr_runp_same; [eapply H| |]; eauto; intros.
+    exploit expr_runp_same; [eapply H0| |]; eauto; intros.
+    eexists; split; eauto. econstructor; eauto.
+  - intros. exploit IHstmnt_runp; eauto; simplify.
+    inversion H3. subst. exploit expr_runp_same; [eapply H| |]; eauto; intros.
+    exploit expr_runp_same; [eapply H0| |]; eauto; intros.
+    eexists; split; eauto. eapply stmnt_runp_Vcase_match; eauto.
+  - intros. exploit IHstmnt_runp; eauto; simplify.
+    inversion H1. subst. exploit expr_runp_same; [eapply H| |]; eauto; intros.
+    eexists; split; eauto. eapply stmnt_runp_Vcase_default; eauto.
+  - inv H; intros.
+    inversion H. subst. exploit expr_runp_same; eauto; intros.
+    econstructor; split; intros. econstructor; eauto. econstructor.
+    econstructor; cbn; eauto.
+    econstructor; intros.
+    destruct (peq r r0); subst.
+    + now rewrite !AssocMap.gss.
+    + rewrite !AssocMap.gso by auto. inv H1; eauto.
+  - inv H; intros.
+    inversion H. subst. exploit expr_runp_same; eauto; intros.
+    econstructor; split; intros. econstructor; eauto. econstructor.
+    econstructor; cbn; eauto.
+    econstructor; intros.
+    destruct (peq r r0); subst.
+    + now rewrite !AssocMap.gss.
+    + rewrite !AssocMap.gso by auto. inv H2; eauto.
+  - inv H; intros. inversion H; subst.
+    exploit expr_runp_same; [eapply H0| |]; eauto; intros.
+    exploit expr_runp_same; [eapply H6| |]; eauto; intros.
+    eexists; split; eauto. econstructor; eauto. econstructor; eauto.
+  - inv H; intros. inversion H; subst.
+    exploit expr_runp_same; [eapply H0| |]; eauto; intros.
+    exploit expr_runp_same; [eapply H6| |]; eauto; intros.
+    eexists; split; eauto. econstructor; eauto. econstructor; eauto.
+Qed.
+
+Lemma exec_ram_same :
+  forall rs1 ar1 c rs2 ar2,
+    exec_ram rs1 ar1 c rs2 ar2 ->
+    forall trs1,
+      match_reg_assocs rs1 trs1 ->
+      exists trs2,
+        exec_ram trs1 ar1 c trs2 ar2
+        /\ match_reg_assocs rs2 trs2.
+Proof.
+  induction 1; intros.
+  - eexists; split; eauto.
+    apply exec_ram_Some_idle. inv H0. cbn in *; setoid_rewrite match_assocmaps_inv_map; eauto.
+  - inv H6; eexists; split; cbn in *.
+    + eapply exec_ram_Some_write. eapply H. eauto. all: cbn in *.
+      now erewrite match_assocmaps_inv_map by eauto.
+      all: now erewrite match_assocmaps_inv by eauto.
+    + unfold nonblock_reg; cbn. constructor; auto.
+      now apply match_assocmaps_set.
+  - inv H5; eexists; split; cbn in *.
+    + eapply exec_ram_Some_read; eauto; cbn in *.
+      now erewrite match_assocmaps_inv_map by eauto.
+      all: now erewrite match_assocmaps_inv by eauto.
+    + unfold nonblock_reg; cbn. constructor; auto.
+      now repeat apply match_assocmaps_set.
+  - eexists; split; cbn in *; eauto. econstructor.
+Qed.
